in progress: adding threads

common/Events.v
@@ -23,77 +23,63 @@ Section EVENTS.
   Variant stateE (V: Type): Type :=
   | SUpdate (run : Any.t -> Any.t * V) : stateE V.
 
+  Variant schE: Type -> Type :=
+  | Spawn (fn: gname) (args: Any.t): schE nat
+  | Yield (tid: nat) : schE unit
+  | Tid : schE nat
+  .
+
   Definition sPut x : stateE unit := SUpdate (fun _ => (x, tt)).
   Definition sGet : stateE Any.t := SUpdate (fun x => (x, x)).
 
-  Definition modE : Type -> Type := (callE +' stateE +' coreE).
-
-  Definition pure_state {S E}: E ~> stateT S (itree E) := fun _ e s => x <- trigger e;; Ret (s, x).
-
-  Lemma unfold_interp_state: forall {E F} {S R} (h: E ~> stateT S (itree F)) (t: itree E R) (s: S),
-    interp_state h t s = _interp_state h (observe t) s.
-  Proof. i. f. apply unfold_interp_state. Qed.  
-
-  Definition handle_stateE {E}: stateE ~> stateT Any.t (itree E) := 
-    fun _ e glob =>
-      match e with
-      | SUpdate run => Ret (run glob)
-      end.
-
-  Definition interp_stateE {E}: itree (stateE +' E) ~> stateT Any.t (itree E) :=
-    (* State.interp_state (case_ ((fun _ e s0 => resum_itr (handle_pE e s0)): _ ~> stateT _ _) State.pure_state). *)
-    State.interp_state (case_ handle_stateE pure_state).
-
-  Definition interp_modE A (prog: callE ~> itree modE) (itr0: itree modE A) (st0: Any.t): itree coreE (Any.t * _)%type :=
-    '(st1, v) <- interp_stateE (interp_mrec prog itr0) st0;;
-    Ret (st1, v).
-
-  Section WRAP.
-
-    Definition assume {E} `{coreE -< E} (P: Prop): itree E unit := trigger (Take P) ;;; Ret tt.
-    Definition guarantee {E} `{coreE -< E} (P: Prop): itree E unit := trigger (Choose P) ;;; Ret tt.
-
-    Definition triggerUB {E A} `{coreE -< E}: itree E A := v <- trigger (Take void);; match v: void with end.
-    Definition triggerNB {E A} `{coreE -< E}: itree E A := v <- trigger (Choose void);; match v: void with end.
-
-    Definition unwrapU {E X} `{coreE -< E} (x: option X): itree E X :=
-      match x with
-      | Some x => Ret x
-      | None => triggerUB
-      end.
-
-    Definition unwrapN {E X} `{coreE -< E} (x: option X): itree E X :=
-      match x with
-      | Some x => Ret x
-      | None => triggerNB
-      end.
-
-    Definition unleftU {E X Y} `{coreE -< E} (xy: X + Y): itree E X :=
-      match xy with
-      | inl x => Ret x
-      | inr y => triggerUB
-      end.
-
-    Definition unleftN {E X Y} `{coreE -< E} (xy: X + Y): itree E X :=
-      match xy with
-      | inl x => Ret x
-      | inr y => triggerNB
-      end.
-
-    Definition unrightU {E X Y} `{coreE -< E} (xy: X + Y): itree E Y :=
-      match xy with
-      | inl x => triggerUB
-      | inr y => Ret y
-      end.
-
-    Definition unrightN {E X Y} `{coreE -< E} (xy: X + Y): itree E Y :=
-      match xy with
-      | inl x => triggerNB
-      | inr y => Ret y
-      end.
-  End WRAP.
+  Definition modE : Type -> Type := schE +' callE +' stateE +' coreE.
 
 End EVENTS.
+
+Section WRAP.
+
+  Definition assume {E} `{coreE -< E} (P: Prop): itree E unit := trigger (Take P) ;;; Ret tt.
+  Definition guarantee {E} `{coreE -< E} (P: Prop): itree E unit := trigger (Choose P) ;;; Ret tt.
+
+  Definition triggerUB {E A} `{coreE -< E}: itree E A := v <- trigger (Take void);; match v: void with end.
+  Definition triggerNB {E A} `{coreE -< E}: itree E A := v <- trigger (Choose void);; match v: void with end.
+
+  Definition unwrapU {E X} `{coreE -< E} (x: option X): itree E X :=
+    match x with
+    | Some x => Ret x
+    | None => triggerUB
+    end.
+
+  Definition unwrapN {E X} `{coreE -< E} (x: option X): itree E X :=
+    match x with
+    | Some x => Ret x
+    | None => triggerNB
+    end.
+
+  Definition unleftU {E X Y} `{coreE -< E} (xy: X + Y): itree E X :=
+    match xy with
+    | inl x => Ret x
+    | inr y => triggerUB
+    end.
+
+  Definition unleftN {E X Y} `{coreE -< E} (xy: X + Y): itree E X :=
+    match xy with
+    | inl x => Ret x
+    | inr y => triggerNB
+    end.
+
+  Definition unrightU {E X Y} `{coreE -< E} (xy: X + Y): itree E Y :=
+    match xy with
+    | inl x => triggerUB
+    | inr y => Ret y
+    end.
+
+  Definition unrightN {E X Y} `{coreE -< E} (xy: X + Y): itree E Y :=
+    match xy with
+    | inl x => triggerNB
+    | inr y => Ret y
+    end.
+End WRAP.
 
 Section EVENTS_OTHER.
 
@@ -113,12 +99,6 @@ Section EVENTS_OTHER.
 
   Definition sf (s: string) (f: string) := (s,f).
 
-  Definition fnsems_scopes {T} (fn: gname) (fnsems: alist gname (list string * T)) :=
-    match (alist_find fn fnsems) with
-    | Some (keys, body) => keys
-    | None => []
-    end.
-
   Inductive pgE: Type -> Type :=
   | SPut (k: key) (v: Any.t): pgE unit
   | SGet (k: key): pgE Any.t.
@@ -127,7 +107,7 @@ Section EVENTS_OTHER.
   | Assume (P: iProp): agE unit
   | Guarantee (P: iProp): agE unit.
 
-  Definition pmodE := callE +' pgE +' coreE.
+  Definition pmodE := schE +' callE +' pgE +' coreE.
   
   Definition hmodE := agE +' pmodE.
 
@@ -169,5 +149,3 @@ Section SYNTAX.
     v <- trigger (SGet k);; (v↓ǃ).
 
 End SYNTAX.
-
-Opaque interp_modE.
