modules/Mod2STS.v
@@ -1,0 +1,386 @@
+Require Import Coqlib.
+Require Export sflib.
+Require Export ITreelib.
+Require Export AList.
+Require Import Events.
+Require Import Skeleton.
+Require Import STS Behavior.
+Require Import Any.
+Require Import Program.
+Require Import Red IRed.
+
+Section EXEC.
+
+  Definition pure_state {S E}: E ~> stateT S (itree E) := fun _ e s => x <- trigger e;; Ret (s, x).
+
+  Lemma unfold_interp_state: forall {E F} {S R} (h: E ~> stateT S (itree F)) (t: itree E R) (s: S),
+    interp_state h t s = _interp_state h (observe t) s.
+  Proof. i. f. apply unfold_interp_state. Qed.
+
+  Definition handle_stateE {E}: stateE ~> stateT Any.t (itree E) :=
+    fun _ e glob =>
+      match e with
+      | SUpdate run => Ret (run glob)
+      end.
+
+  Definition interp_stateE {E}: itree (stateE +' E) ~> stateT Any.t (itree E) :=
+    State.interp_state (case_ handle_stateE pure_state).
+
+  Definition ths_state : Type := nat * list (itree modE Any.t).
+
+  Definition handle_schE_callE (prog: callE ~> itree modE):
+    ths_state -> itree (stateE +' coreE) (ths_state + Any.t) :=
+    fun '(tid, ths) =>
+      match base.lookup tid ths with
+      | None => Ret (inl (0, ths))
+      | Some itr =>
+          match observe (itr: itree modE Any.t) with
+          | RetF rv =>
+              if Nat.eq_dec tid 0 then Ret (inr rv) else Ret (inl (0, ths))
+          | TauF itr' =>
+              tau;; Ret (inl (tid, base.insert tid itr' ths))
+          | VisF (inr1 (inr1 e)) k =>
+              v <- trigger e;;
+              Ret (inl (tid, base.insert tid (k v) ths))
+          | VisF (inr1 (inl1 e)) k =>
+              Ret (inl (tid, base.insert tid (prog _ e >>= k) ths))
+          | VisF (inl1 e) k =>
+              match e in schE T return (T -> _) -> _ with
+              | Spawn fn arg => fun k =>
+                  Ret (inl (tid, (base.insert tid (k (List.length ths)) ths) ++ [prog _ (Call fn arg)]))
+              | Yield tid' => fun k =>
+                  Ret (inl (tid', base.insert tid (k tt) ths))
+              | Tid => fun k =>
+                  Ret (inl (tid, base.insert tid (k tid) ths))
+              end k
+          end
+      end.
+
+  Definition interp_schE_callE (prog: callE ~> itree modE) (itr0: itree modE Any.t)
+    : itree (stateE +' coreE) Any.t
+    :=
+    ITree.iter (handle_schE_callE prog) (0, [itr0]).
+
+  Definition interp_modE (prog: callE ~> itree modE) (itr0: itree modE Any.t) (st0: Any.t): itree coreE _ :=
+    interp_stateE Any.t (interp_schE_callE prog itr0) st0.
+
+End EXEC.
+
+(*
+Opaque interp_modE.
+
+Section RED.
+
+  Variable prog: callE ~> itree modE.
+
+  Lemma interp_modE_bind
+        A
+        (itr: itree modE A) (ktr: A -> itree modE Any.t)
+        st0
+    :
+      interp_modE prog (v <- itr ;; ktr v) st0 =
+      '(st1, v) <- interp_modE prog (itr) st0 ;; interp_modE prog (ktr v) st1.
+
+  Proof. unfold interp_modE, interp_stateE. des_ifs. grind. Qed.
+
+  Lemma interp_modE_tau
+        (prog: callE ~> itree modE)
+        A
+        (itr: itree modE A)
+        st0
+    :
+      interp_modE prog (tau;; itr) st0 = tau;; interp_modE prog itr st0.
+  Proof. unfold interp_modE, interp_stateE. des_ifs. grind. Qed.
+
+  Lemma interp_modE_ret
+        T
+        prog st0 (v: T)
+    :
+      interp_modE prog (Ret v: itree modE _) st0 = Ret (st0, v).
+  Proof. unfold interp_modE, interp_stateE. des_ifs. grind. Qed.
+
+  Lemma interp_modE_callE
+        p st0 T
+        (* (e: modE Σ) *)
+        (e: callE T)
+    :
+      interp_modE p (trigger e) st0 = tau;; (interp_modE p (p _ e) st0).
+  Proof. unfold interp_modE, interp_stateE. des_ifs. grind. Qed.
+
+  Lemma interp_modE_stateE
+        p st0
+        (* (e: modE Σ) *)
+        T
+        (e: stateE T)
+    :
+      interp_modE p (trigger e) st0 =
+      '(st1, r) <- handle_stateE e st0;;
+      tau;; tau;;
+      Ret (st1, r).
+  Proof.
+    unfold interp_modE, interp_stateE. grind.
+  Qed.
+
+  Lemma interp_modE_coreE
+        p st0
+        T
+        (e: coreE T)
+    :
+      interp_modE p (trigger e) st0 = r <- trigger e;; tau;; tau;; Ret (st0, r).
+  Proof.
+    unfold interp_modE, interp_stateE. grind.
+    unfold pure_state. grind.
+  Qed.
+
+  Lemma interp_modE_triggerUB
+        (prog: callE ~> itree modE)
+        st0
+        A
+    :
+      (interp_modE prog (triggerUB) st0: itree coreE (_ * A)) = triggerUB.
+  Proof.
+    unfold interp_modE, interp_stateE, pure_state, triggerUB. grind.
+  Qed.
+
+  Lemma interp_modE_triggerNB
+        (prog: callE ~> itree modE)
+        st0
+        A
+    :
+      (interp_modE prog (triggerNB) st0: itree coreE (_ * A)) = triggerNB.
+  Proof.
+    unfold interp_modE, interp_stateE, pure_state, triggerNB. grind.
+  Qed. 
+  
+  Lemma interp_modE_unwrapU
+        prog R st0 (r: option R)
+    :
+      interp_modE prog (unwrapU r) st0 = r <- unwrapU r;; Ret (st0, r).
+  Proof.
+    unfold unwrapU. des_ifs.
+    - rewrite interp_modE_ret. grind.
+    - rewrite interp_modE_triggerUB. unfold triggerUB. grind.
+  Qed.
+
+  Lemma interp_modE_unwrapN
+        prog R st0 (r: option R)
+    :
+      interp_modE prog (unwrapN r) st0 = r <- unwrapN r;; Ret (st0, r).
+  Proof.
+    unfold unwrapN. des_ifs.
+    - rewrite interp_modE_ret. grind.
+    - rewrite interp_modE_triggerNB. unfold triggerNB. grind.
+  Qed.
+
+  Lemma interp_modE_assume
+        prog st0 (P: Prop)
+    :
+      interp_modE prog (assume P) st0 = assume P;;; tau;; tau;; Ret (st0, tt).
+  Proof.
+    unfold assume.
+    repeat (try rewrite interp_modE_bind; try rewrite bind_bind). grind.
+    rewrite interp_modE_coreE.
+    repeat (try rewrite interp_modE_bind; try rewrite bind_bind). grind.
+    rewrite interp_modE_ret.
+    refl.
+  Qed.
+
+  Lemma interp_modE_guarantee
+        prog st0 (P: Prop)
+    :
+      interp_modE prog (guarantee P) st0 = guarantee P;;; tau;; tau;; Ret (st0, tt).
+  Proof.
+    unfold guarantee.
+    repeat (try rewrite interp_modE_bind; try rewrite bind_bind). grind.
+    rewrite interp_modE_coreE.
+    repeat (try rewrite interp_modE_bind; try rewrite bind_bind). grind.
+    rewrite interp_modE_ret.
+    refl.
+  Qed.    
+
+  Lemma interp_modE_ext
+        prog R (itr0 itr1: itree _ R) st0
+    : 
+      itr0 = itr1 -> interp_modE prog itr0 st0 = interp_modE prog itr1 st0.
+  Proof. i; subst; refl. Qed.    
+
+End RED.
+
+Global Program Instance interp_modE_rdb: red_database (mk_box (@interp_modE)) :=
+  mk_rdb
+    1
+    (mk_box interp_modE_bind)
+    (mk_box interp_modE_tau)
+    (mk_box interp_modE_ret)
+    (mk_box interp_modE_stateE)
+    (mk_box interp_modE_stateE)
+    (mk_box interp_modE_callE)
+    (mk_box interp_modE_coreE)
+    (mk_box interp_modE_triggerUB)
+    (mk_box interp_modE_triggerNB)
+    (mk_box interp_modE_unwrapU)
+    (mk_box interp_modE_unwrapN)
+    (mk_box interp_modE_assume)
+    (mk_box interp_modE_guarantee)
+    (mk_box interp_modE_ext).
+
+ *)
+
+Section SEMANTICS.
+  Let state: Type := itree coreE Any.t.
+
+  Definition state_sort (st0: state): sort :=
+    match (observe st0) with
+    | TauF _ => demonic
+    | RetF rv => final rv
+    | VisF (Choose X) k => demonic
+    | VisF (Take X) k => angelic
+    | VisF (IO fn args) k => STS.vis
+    end.
+
+  Inductive step: state -> option event -> state -> Prop :=
+  | step_tau
+      itr
+    :
+      step (Tau itr) None itr
+  | step_choose
+      X k (x: X)
+    :
+      step (Vis (subevent _ (Choose X)) k) None (k x)
+  | step_take
+      X k (x: X)
+    :
+      step (Vis (subevent _ (Take X)) k) None (k x)
+  | step_io
+      fn I O (args: I) (rv: O) k
+    :
+      step (Vis (subevent _ (IO fn args)) k) (Some (event_io fn args rv)) (k rv).
+
+  Lemma step_trigger_choose_iff X k itr e
+        (STEP: step (trigger (Choose X) >>= k) e itr)
+    :
+      exists x,
+        e = None /\ itr = k x.
+  Proof.
+    inv STEP.
+    { eapply f_equal with (f:=observe) in H0. ss. }
+    { eapply f_equal with (f:=observe) in H0. ss.
+      unfold trigger in H0. ss. cbn in H0.
+      dependent destruction H0. ired. et.  }
+    { eapply f_equal with (f:=observe) in H0. ss. }
+    { eapply f_equal with (f:=observe) in H0. ss. }
+  Qed.
+
+  Lemma step_trigger_take_iff X k itr e
+        (STEP: step (trigger (Take X) >>= k) e itr)
+    :
+      exists x,
+        e = None /\ itr = k x.
+  Proof.
+    inv STEP.
+    { eapply f_equal with (f:=observe) in H0. ss. }
+    { eapply f_equal with (f:=observe) in H0. ss. }
+    { eapply f_equal with (f:=observe) in H0. ss.
+      unfold trigger in H0. ss. cbn in H0.
+      dependent destruction H0. ired. et.  }
+    { eapply f_equal with (f:=observe) in H0. ss. }
+  Qed.
+
+  Lemma step_tau_iff itr0 itr1 e
+        (STEP: step (Tau itr0) e itr1)
+    :
+      e = None /\ itr0 = itr1.
+  Proof.
+    inv STEP. et.
+  Qed.
+
+  Lemma step_ret_iff rv itr e
+        (STEP: step (Ret rv) e itr)
+    :
+      False.
+  Proof.
+    inv STEP.
+  Qed.
+
+  Lemma step_trigger_io_iff fn I O args k e itr
+        (STEP: step (trigger (@IO I O fn args) >>= k) e itr)
+    :
+      exists rv, itr = k rv /\ e = Some (event_io fn args rv).
+  Proof.
+    inv STEP.
+    { eapply f_equal with (f:=observe) in H0. ss. }
+    { eapply f_equal with (f:=observe) in H0. ss. }
+    { eapply f_equal with (f:=observe) in H0. ss. }
+    { eapply f_equal with (f:=observe) in H0. ss.
+      unfold trigger in H0. ss. cbn in H0.
+      dependent destruction H0. ired. et. }
+  Qed.
+
+  Let itree_eta E R (itr0 itr1: itree E R)
+      (OBSERVE: observe itr0 = observe itr1)
+    :
+      itr0 = itr1.
+  Proof.
+    rewrite (itree_eta_ itr0).
+    rewrite (itree_eta_ itr1).
+    rewrite OBSERVE. auto.
+  Qed.
+
+  Lemma step_trigger_choose X k x
+    :
+      step (trigger (Choose X) >>= k) None (k x).
+  Proof.
+    unfold trigger. ss.
+    match goal with
+    | [ |- step ?itr _ _] =>
+      replace itr with (Subevent.vis (Choose X) k)
+    end; ss.
+    { econs. }
+    { eapply itree_eta. ss. cbv. f_equal.
+      extensionality x0. eapply itree_eta. ss. }
+  Qed.
+
+  Lemma step_trigger_take X k x
+    :
+      step (trigger (Take X) >>= k) None (k x).
+  Proof.
+    unfold trigger. ss.
+    match goal with
+    | [ |- step ?itr _ _] =>
+      replace itr with (Subevent.vis (Take X) k)
+    end; ss.
+    { econs. }
+    { eapply itree_eta. ss. cbv. f_equal.
+      extensionality x0. eapply itree_eta. ss. }
+  Qed.
+
+  Lemma step_trigger_io I O fn (args: I) k (rv: O)
+    :
+      step (trigger (IO fn args) >>= k) (Some (event_io fn args rv)) (k rv).
+  Proof.
+    unfold trigger. ss.
+    match goal with
+    | [ |- step ?itr _ _] =>
+      replace itr with (Subevent.vis (IO fn args) k)
+    end; ss.
+    { econs; et. }
+    { eapply itree_eta. ss. cbv. f_equal.
+      extensionality x0. eapply itree_eta. ss. }
+  Qed.
+
+
+  Program Definition compile_itree: itree coreE Any.t -> semantics :=
+    fun itr =>
+      {|
+        STS.state := state;
+        STS.step := step;
+        STS.initial_state := itr;
+        STS.state_sort := state_sort;
+      |}.
+  Next Obligation. inv STEP; inv STEP0; ss. csc. Qed.
+  Next Obligation. inv STEP; ss. Qed.
+  Next Obligation. inv STEP; ss. Qed.
+  Next Obligation. inv STEP; ss. Qed.
+  Next Obligation. inv STEP; ss. Qed.
+  
+End SEMANTICS.
